More proofs

inductive_proof/Queue_set/App.fst
@@ -6,7 +6,7 @@ module S = Set_extended
 #set-options "--query_stats"
 // the concrete state type
 // It is a set of pairs of timestamp and element.
-type concrete_st = s:S.set (nat & nat)//{s <> empty ==> (exists (e:(nat * nat)). mem e s /\ (forall e1. mem e1 s ==> fst e <= fst e1))}
+type concrete_st = S.set (nat & nat)//{s <> empty ==> (exists (e:(nat * nat)). mem e s /\ (forall e1. mem e1 s ==> fst e <= fst e1))}
 
 // init state
 let init_st = S.empty
@@ -40,67 +40,44 @@ let get_ele (o:op_t{Enqueue? (fst (snd o))}) : nat =
   match o with
   |(_, (Enqueue x,_)) -> x
 
-let mem_id_s (id:nat) (s:concrete_st) =
-  S.exists_s s (fun e -> fst e = id)
-  
-let unique_st (s:concrete_st) =
-  //forall_s s (fun e -> count e s > 0) &&
-  S.forall_s s (fun e -> not (S.exists_s s (fun e1 -> snd e <> snd e1 && fst e = fst e1)))
-
-val extract_s (#a:Type0) (m:option a{Some? m}) : a
-let extract_s (Some x) = x
-
-let find_min (s:concrete_st)
-    : (m:option (nat * nat) 
-           {(Some? m <==> (exists (e:(nat * nat)). S.mem e s /\ (forall e1. S.mem e1 s ==> fst e <= fst e1))) /\
-            (Some? m ==> (exists (e:(nat * nat)). S.mem e s /\ (forall e1. S.mem e1 s ==> fst e <= fst e1) /\ e = extract_s m)) /\
-        (s = S.empty ==> (m = None \/ (~ (exists (e:(nat * nat)). S.mem e s /\ (forall e1. S.mem e1 s ==> fst e <= fst e1))))) 
-        (*s <> empty ==> Some? m*)}) =
-  S.find_if s (fun e -> (S.forall_s s (fun e1 -> fst e <= fst e1)))
-
 let check_find_min (s:concrete_st)
   : Lemma (requires s = S.add (2,1) (S.singleton (3,1)))
-          (ensures find_min s = Some (2,1)) 
-  = let m = find_min s in
+          (ensures S.find_min s = Some (2,1)) 
+  = let m = S.find_min s in
     assert (S.mem (2,1) s /\ (forall e1. S.mem e1 s ==> fst (2,1) <= fst e1));
     (*assert (Some? m);
     assert (fst (extract_s m) = 1);
     assert (forall e. mem e s ==> 1 <= fst e);*) ()
 
-let remove_min (s:concrete_st) 
-  : (r:concrete_st{(s = S.empty ==> r = s) /\
-                   (s <> S.empty /\ Some? (find_min s) ==> (forall e. S.mem e r <==> (S.mem e s /\ e <> extract_s (find_min s)))) /\
-                   (s <> S.empty /\ None? (find_min s) ==> (forall e. S.mem e r <==> S.mem e s))}) =
-  if s = S.empty then s 
-  else (let m = find_min s in
-        if Some? m then S.remove_if s (fun e -> e = extract_s (find_min s))
-        else s)
-
-let find_min_equal (a b:concrete_st)
-  : Lemma (requires unique_st a /\ unique_st b /\ eq a b)
-          (ensures eq (remove_min a) (remove_min b)) = ()
-
 // apply an operation to a state
 let do (s:concrete_st) (op:op_t) : concrete_st =
   match op with
   |(id, (Enqueue x, _)) -> S.add (id, x) s
-  |(_, (Dequeue, _)) -> if s = S.empty then s else remove_min s
+  |(_, (Dequeue, _)) -> if s = S.empty then s else S.remove_min s
+
+let eq_min_same (a b:concrete_st) 
+  : Lemma (requires eq a b /\ S.unique_st a /\ S.unique_st b)
+          (ensures S.find_min a = S.find_min b) = ()
 
 let lem_do (a b:concrete_st) (op:op_t)
    : Lemma (requires eq a b)
            (ensures eq (do a op) (do b op)) = 
-  assume (unique_st a /\ unique_st b); 
-  match op with
-  |(id, (Enqueue x, _)) -> ()
-  |(_, (Dequeue, _)) -> ()
+  assume (S.unique_st a /\ S.unique_st b);
+  eq_min_same a b;
+  if Enqueue? (fst (snd op)) then () else ()
   
 let return (s:concrete_st) (o:op_t) : ret_t =
   match o with
   |(_, (Enqueue _, _)) -> None
   |(_, (Dequeue, r)) -> if s = S.empty then None 
-                          else (assume (exists (e:(nat * nat)). S.mem e s /\ (forall e1. S.mem e1 s ==> fst e <= fst e1));
-                                assert (Some? (find_min s));
-                                Some (extract_s (find_min s)))
+                          else (S.always_min_exists s; 
+                                assert (Some? (S.find_min s));
+                                Some (S.extract_s (S.find_min s)))
+
+let last_deq (s:concrete_st) (op:op_t)
+  : Lemma (requires Dequeue? (fst (snd op)) /\ Some? (ret_of op) /\ return s op == ret_of op)
+          (ensures s <> S.empty /\ S.find_min s == ret_of op /\
+                   S.mem (S.extract_s (S.find_min s)) s) = S.always_min_exists s
 
 let extract (o:op_t{Dequeue? (fst (snd o)) /\ Some? (ret_of o)}) : (nat * nat) =
   let (_, (_, Some x)) = o in x
@@ -114,7 +91,7 @@ let resolve_conflict (x:op_t) (y:op_t{fst x <> fst y}) : resolve_conflict_res =
   |(_,(Dequeue,None)), (_,(Dequeue,None)) -> Noop_both
   |(_,(Enqueue _,_)), (_,(Dequeue,Some _)) -> Second_then_first
   |(_,(Dequeue,Some _)), (_,(Enqueue _,_)) -> First_then_second 
-  |(_,(Dequeue,Some _)), (_,(Dequeue,Some _)) -> if fst (extract x) = fst (extract y) then First 
+  |(_,(Dequeue,Some _)), (_,(Dequeue,Some _)) -> if extract x = extract y then First 
                                                  else if fst (extract x) < fst (extract y) then First_then_second
                                                       else Second_then_first
  
@@ -127,6 +104,47 @@ let concrete_merge (lca s1 s2:concrete_st)
   let da = S.remove_if s1 (fun e -> S.mem e lca) in
   let db = S.remove_if s2 (fun e -> S.mem e lca) in
   S.union i (S.union da db)
+
+let do_is_unique (s:concrete_st) (op:op_t) 
+  : Lemma (requires S.unique_st s /\ (not (S.mem_id_s (fst op) s)))
+          (ensures S.unique_st (do s op)) = 
+  match op with
+  |(id, (Enqueue x, _)) -> ()
+  |(_, (Dequeue, _)) -> ()
+
+let append_id (l:concrete_st) (ele:(nat * nat))
+  : Lemma (ensures (forall id. S.mem_id_s id (S.add ele l) <==> S.mem_id_s id l \/ id = fst ele) /\
+                   (S.unique_st l /\ not (S.mem_id_s (fst ele) l)) ==> 
+                    S.unique_st (S.add ele l))
+  = ()
+
+let rec lem_foldl (s:concrete_st) (l:log)
+  : Lemma (requires true)
+          (ensures (forall id. S.mem_id_s id (apply_log s l) ==> S.mem_id_s id s \/ mem_id id l))
+          (decreases length l) =
+  match length l with
+  |0 -> ()
+  |_ -> (if Enqueue? (fst (snd (head l))) then append_id s (fst (head l), get_ele (head l)) else ());
+       mem_cons (head l) (tail l);
+       lem_foldl (do s (head l)) (tail l)
+       
+let rec lem_foldl1 (s:concrete_st) (l:log)
+  : Lemma (requires S.unique_st s /\ distinct_ops l /\
+                    (forall id. S.mem_id_s id s ==> not (mem_id id l)))
+          (ensures S.unique_st (apply_log s l))
+          (decreases length l) =
+  match length l with
+  |0 -> ()
+  |_ -> do_is_unique s (head l);
+       (if Enqueue? (fst (snd (head l))) then append_id s (fst (head l), get_ele (head l)) else ());
+       mem_cons (head l) (tail l);
+       distinct_invert_append (create 1 (head l)) (tail l);
+       lem_foldl1 (do s (head l)) (tail l)
+
+let valid_is_unique (s:st0) 
+  : Lemma (requires distinct_ops (ops_of s) /\ v_of s == apply_log init_st (ops_of s))
+          (ensures S.unique_st (v_of s)) =
+  lem_foldl1 init_st (ops_of s)
   
 let linearizable_s1_0''_base_base (lca s1 s2':st) (last2:op_t)
   : Lemma (requires consistent_branches lca s1 s2' /\
@@ -240,11 +258,11 @@ let linearizable_gt0_base_de_fts (lca s1 s2:st) (last1 last2:op_t)
          
           (ensures (eq (do (concrete_merge (v_of lca) (v_of s1) (do (v_of s2) last2)) last1)
                        (concrete_merge (v_of lca) (do (v_of s1) last1) (do (v_of s2) last2)))) = 
-  assume (unique_st (v_of lca) /\ unique_st (v_of s1) /\ unique_st (v_of s2)); //todo
+  valid_is_unique lca; valid_is_unique s1; valid_is_unique s2;
   assume (ret_of last1 = return (v_of s1) last1); //to include in pre-cond    
   assume (ret_of last2 = return (v_of s2) last2); //to include in pre-cond  
-  assume (forall id. mem_id_s id (v_of s2) ==> fst last2 > id);
-  ()
+  assume (forall id. S.mem_id_s id (v_of s2) ==> fst last2 > id);
+  admit()
 
 let linearizable_gt0_base_dd_fts (lca s1 s2:st) (last1 last2:op_t)
   : Lemma (requires consistent_branches lca s1 s2 /\
@@ -259,7 +277,7 @@ let linearizable_gt0_base_dd_fts (lca s1 s2:st) (last1 last2:op_t)
          
           (ensures (eq (do (concrete_merge (v_of lca) (v_of s1) (do (v_of s2) last2)) last1)
                        (concrete_merge (v_of lca) (do (v_of s1) last1) (do (v_of s2) last2)))) = 
-  assume (unique_st (v_of lca) /\ unique_st (v_of s1) /\ unique_st (v_of s2)); //todo
+  valid_is_unique lca; valid_is_unique s1; valid_is_unique s2;
   assume (ret_of last1 = return (v_of s1) last1); //to include in pre-cond    
   assume (ret_of last2 = return (v_of s2) last2); //to include in pre-cond  
   ()
@@ -303,11 +321,11 @@ let linearizable_gt0_base_de_stf (lca s1 s2:st) (last1 last2:op_t)
          
           (ensures eq (do (concrete_merge (v_of lca) (do (v_of s1) last1) (v_of s2)) last2)
                       (concrete_merge (v_of lca) (do (v_of s1) last1) (do (v_of s2) last2))) = 
-  assume (unique_st (v_of lca) /\ unique_st (v_of s1) /\ unique_st (v_of s2)); //todo
+  valid_is_unique lca; valid_is_unique s1; valid_is_unique s2;
   assume (ret_of last1 = return (v_of s1) last1); //to include in pre-cond    
   assume (ret_of last2 = return (v_of s2) last2); //to include in pre-cond  
-  assume (forall id. mem_id_s id (v_of s1) ==> fst last1 > id);
-  ()
+  assume (forall id. S.mem_id_s id (v_of s1) ==> fst last1 > id);
+  admit()
 
 let linearizable_gt0_base_dd_stf (lca s1 s2:st) (last1 last2:op_t)
   : Lemma (requires consistent_branches lca s1 s2 /\
@@ -322,7 +340,7 @@ let linearizable_gt0_base_dd_stf (lca s1 s2:st) (last1 last2:op_t)
          
           (ensures eq (do (concrete_merge (v_of lca) (do (v_of s1) last1) (v_of s2)) last2)
                       (concrete_merge (v_of lca) (do (v_of s1) last1) (do (v_of s2) last2))) = 
-   assume (unique_st (v_of lca) /\ unique_st (v_of s1) /\ unique_st (v_of s2)); //todo
+   valid_is_unique lca; valid_is_unique s1; valid_is_unique s2;
    assume (ret_of last1 = return (v_of s1) last1); //to include in pre-cond    
    assume (ret_of last2 = return (v_of s2) last2); //to include in pre-cond  
    ()
@@ -356,7 +374,217 @@ let linearizable_gt0_base (lca s1 s2:st) (last1 last2:op_t)
 
                    (Second_then_first? (resolve_conflict last1 last2) ==>
                       (eq (do (concrete_merge (v_of lca) (do (v_of s1) last1) (v_of s2)) last2)
-                         (concrete_merge (v_of lca) (do (v_of s1) last1) (do (v_of s2) last2))))) = admit()
+                         (concrete_merge (v_of lca) (do (v_of s1) last1) (do (v_of s2) last2))))) =
+  if First_then_second? (resolve_conflict last1 last2) then
+    linearizable_gt0_base_fts lca s1 s2 last1 last2
+  else if Second_then_first? (resolve_conflict last1 last2) then 
+    linearizable_gt0_base_stf lca s1 s2 last1 last2
+  else ()
+
+let linearizable_gt0_ind_ee_fts (lca s1 s2:st) (last1 last2:op_t)
+  : Lemma (requires consistent_branches_s2_gt0 lca s1 s2 /\
+                    fst last1 <> fst last2 /\
+                    distinct_ops (snoc (ops_of s1) last1) /\
+                    distinct_ops (snoc (ops_of s2) last2) /\
+                    (exists l1. (do (v_of s1) last1 == apply_log (v_of lca) l1)) /\
+                    (exists l2. (do (v_of s2) last2 == apply_log (v_of lca) l2)) /\
+                    (let s2' = inverse_st s2 in
+                    (exists l2. (do (v_of s2') last2 == apply_log (v_of lca) l2)) /\
+                    (exists l2. (v_of s2' == apply_log (v_of lca) l2)) /\
+                    (exists l1. (v_of s1 == apply_log (v_of lca) l1)) /\
+                    (exists l2. (v_of s2 == apply_log (v_of lca) l2)) /\
+                    consistent_branches lca s1 s2' /\
+                    First_then_second? (resolve_conflict last1 last2) /\
+                    Enqueue? (fst (snd last1)) /\ Enqueue? (fst (snd last2)) /\ fst last1 > fst last2 /\
+                    eq (do (concrete_merge (v_of lca) (v_of s1) (do (v_of s2') last2)) last1)
+                       (concrete_merge (v_of lca) (do (v_of s1) last1) (do (v_of s2') last2))))
+       
+          (ensures eq (do (concrete_merge (v_of lca) (v_of s1) (do (v_of s2) last2)) last1)
+                      (concrete_merge (v_of lca) (do (v_of s1) last1) (do (v_of s2) last2))) = 
+   assume (forall id. S.mem_id_s id (v_of lca) ==> fst last1 > id); //todo
+   ()
+
+#push-options "--z3rlimit 200"
+let linearizable_gt0_ind_de_fts (lca s1 s2:st) (last1 last2:op_t)
+  : Lemma (requires consistent_branches_s2_gt0 lca s1 s2 /\
+                    fst last1 <> fst last2 /\
+                    distinct_ops (snoc (ops_of s1) last1) /\
+                    distinct_ops (snoc (ops_of s2) last2) /\
+                    (exists l1. (do (v_of s1) last1 == apply_log (v_of lca) l1)) /\
+                    (exists l2. (do (v_of s2) last2 == apply_log (v_of lca) l2)) /\
+                    (let s2' = inverse_st s2 in
+                    (exists l2. (do (v_of s2') last2 == apply_log (v_of lca) l2)) /\
+                    (exists l2. (v_of s2' == apply_log (v_of lca) l2)) /\
+                    (exists l1. (v_of s1 == apply_log (v_of lca) l1)) /\
+                    (exists l2. (v_of s2 == apply_log (v_of lca) l2)) /\
+                    consistent_branches lca s1 s2' /\
+                    First_then_second? (resolve_conflict last1 last2) /\
+                    Dequeue? (fst (snd last1)) /\ Some? (ret_of last1) /\ Enqueue? (fst (snd last2)) /\
+                    eq (do (concrete_merge (v_of lca) (v_of s1) (do (v_of s2') last2)) last1)
+                       (concrete_merge (v_of lca) (do (v_of s1) last1) (do (v_of s2') last2))))
+       
+          (ensures eq (do (concrete_merge (v_of lca) (v_of s1) (do (v_of s2) last2)) last1)
+                      (concrete_merge (v_of lca) (do (v_of s1) last1) (do (v_of s2) last2))) = 
+  admit()
+
+let linearizable_gt0_ind_dd_fts (lca s1 s2:st) (last1 last2:op_t)
+  : Lemma (requires consistent_branches_s2_gt0 lca s1 s2 /\
+                    fst last1 <> fst last2 /\
+                    distinct_ops (snoc (ops_of s1) last1) /\
+                    distinct_ops (snoc (ops_of s2) last2) /\
+                    (exists l1. (do (v_of s1) last1 == apply_log (v_of lca) l1)) /\
+                    (exists l2. (do (v_of s2) last2 == apply_log (v_of lca) l2)) /\
+                    (let s2' = inverse_st s2 in
+                    (exists l2. (do (v_of s2') last2 == apply_log (v_of lca) l2)) /\
+                    (exists l2. (v_of s2' == apply_log (v_of lca) l2)) /\
+                    (exists l1. (v_of s1 == apply_log (v_of lca) l1)) /\
+                    (exists l2. (v_of s2 == apply_log (v_of lca) l2)) /\
+                    consistent_branches lca s1 s2' /\
+                    First_then_second? (resolve_conflict last1 last2) /\
+                    Dequeue? (fst (snd last1)) /\ Some? (ret_of last1) /\ 
+                    Dequeue? (fst (snd last2)) /\ Some? (ret_of last2) /\
+                    fst (extract last1) < fst (extract last2) /\
+                    eq (do (concrete_merge (v_of lca) (v_of s1) (do (v_of s2') last2)) last1)
+                       (concrete_merge (v_of lca) (do (v_of s1) last1) (do (v_of s2') last2))))
+       
+          (ensures eq (do (concrete_merge (v_of lca) (v_of s1) (do (v_of s2) last2)) last1)
+                      (concrete_merge (v_of lca) (do (v_of s1) last1) (do (v_of s2) last2))) = 
+  valid_is_unique lca; valid_is_unique s1; valid_is_unique s2;
+  assume (ret_of last1 = return (v_of s1) last1); //to include in pre-cond    
+  assume (ret_of last2 = return (v_of s2) last2); //to include in pre-cond  
+  last_deq (v_of s1) last1;
+  last_deq (v_of s2) last2;
+     //assume (forall e. S.mem e (v_of s1) /\ S.mem e (do (v_of s2) last2) ==> S.mem e (v_of lca));
+     //assume (forall e. S.mem e (do (v_of s1) last1) /\ S.mem e (do (v_of s2) last2) ==> S.mem e (v_of lca));
+     //assume (fst (extract_s (find_min (v_of s1))) < fst (extract_s (find_min (v_of s2))));
+  let s2' = inverse_st s2 in
+  assume (S.find_min (concrete_merge (v_of lca) (do (v_of s1) last1) (do (v_of s2') last2)) = (S.find_min (v_of s1)));
+  assert (S.find_min (concrete_merge (v_of lca) (v_of s1) (do (v_of s2) last2)) = (S.find_min (v_of s1)));
+  ()
+
+let linearizable_gt0_ind_fts (lca s1 s2:st) (last1 last2:op_t)
+  : Lemma (requires consistent_branches_s2_gt0 lca s1 s2 /\
+                    fst last1 <> fst last2 /\
+                    distinct_ops (snoc (ops_of s1) last1) /\
+                    distinct_ops (snoc (ops_of s2) last2) /\
+                    (exists l1. (do (v_of s1) last1 == apply_log (v_of lca) l1)) /\
+                    (exists l2. (do (v_of s2) last2 == apply_log (v_of lca) l2)) /\
+                    (let s2' = inverse_st s2 in
+                    (exists l2. (do (v_of s2') last2 == apply_log (v_of lca) l2)) /\
+                    (exists l2. (v_of s2' == apply_log (v_of lca) l2)) /\
+                    (exists l1. (v_of s1 == apply_log (v_of lca) l1)) /\
+                    (exists l2. (v_of s2 == apply_log (v_of lca) l2)) /\
+                    consistent_branches lca s1 s2' /\
+                    First_then_second? (resolve_conflict last1 last2) /\
+                    eq (do (concrete_merge (v_of lca) (v_of s1) (do (v_of s2') last2)) last1)
+                       (concrete_merge (v_of lca) (do (v_of s1) last1) (do (v_of s2') last2))))
+          (ensures eq (do (concrete_merge (v_of lca) (v_of s1) (do (v_of s2) last2)) last1)
+                        (concrete_merge (v_of lca) (do (v_of s1) last1) (do (v_of s2) last2)))
+          [SMTPat (eq (do (concrete_merge (v_of lca) (v_of s1) (do (v_of s2) last2)) last1)
+                      (concrete_merge (v_of lca) (do (v_of s1) last1) (do (v_of s2) last2)))]             =
+  if Enqueue? (fst (snd last1)) && Enqueue? (fst (snd last2)) && fst last1 > fst last2 then
+    linearizable_gt0_ind_ee_fts lca s1 s2 last1 last2
+  else if Dequeue? (fst (snd last1)) && Some? (ret_of last1) && Enqueue? (fst (snd last2)) then
+    linearizable_gt0_ind_de_fts lca s1 s2 last1 last2
+  else linearizable_gt0_ind_dd_fts lca s1 s2 last1 last2
+
+let linearizable_gt0_ind_ee_stf (lca s1 s2:st) (last1 last2:op_t)
+  : Lemma (requires consistent_branches_s2_gt0 lca s1 s2 /\
+                    fst last1 <> fst last2 /\
+                    distinct_ops (snoc (ops_of s1) last1) /\
+                    distinct_ops (snoc (ops_of s2) last2) /\
+                    (exists l1. (do (v_of s1) last1 == apply_log (v_of lca) l1)) /\
+                    (exists l2. (do (v_of s2) last2 == apply_log (v_of lca) l2)) /\
+                    (let s2' = inverse_st s2 in
+                    (exists l2. (do (v_of s2') last2 == apply_log (v_of lca) l2)) /\
+                    (exists l2. (v_of s2' == apply_log (v_of lca) l2)) /\
+                    (exists l1. (v_of s1 == apply_log (v_of lca) l1)) /\
+                    (exists l2. (v_of s2 == apply_log (v_of lca) l2)) /\
+                    consistent_branches lca s1 s2' /\
+                    ops_of s1 = ops_of lca /\
+                    Second_then_first? (resolve_conflict last1 last2) /\
+                    Enqueue? (fst (snd last1)) /\ Enqueue? (fst (snd last2)) /\ fst last1 < fst last2 /\
+                    eq (do (concrete_merge (v_of lca) (do (v_of s1) last1) (v_of s2')) last2)
+                       (concrete_merge (v_of lca) (do (v_of s1) last1) (do (v_of s2') last2))))
+          (ensures eq (do (concrete_merge (v_of lca) (do (v_of s1) last1) (v_of s2)) last2)
+                      (concrete_merge (v_of lca) (do (v_of s1) last1) (do (v_of s2) last2))) = ()
+
+let linearizable_gt0_ind_de_stf (lca s1 s2:st) (last1 last2:op_t)
+  : Lemma (requires consistent_branches_s2_gt0 lca s1 s2 /\
+                    fst last1 <> fst last2 /\
+                    distinct_ops (snoc (ops_of s1) last1) /\
+                    distinct_ops (snoc (ops_of s2) last2) /\
+                    (exists l1. (do (v_of s1) last1 == apply_log (v_of lca) l1)) /\
+                    (exists l2. (do (v_of s2) last2 == apply_log (v_of lca) l2)) /\
+                    (let s2' = inverse_st s2 in
+                    (exists l2. (do (v_of s2') last2 == apply_log (v_of lca) l2)) /\
+                    (exists l2. (v_of s2' == apply_log (v_of lca) l2)) /\
+                    (exists l1. (v_of s1 == apply_log (v_of lca) l1)) /\
+                    (exists l2. (v_of s2 == apply_log (v_of lca) l2)) /\
+                    consistent_branches lca s1 s2' /\
+                    ops_of s1 = ops_of lca /\
+                    Second_then_first? (resolve_conflict last1 last2) /\
+                    Dequeue? (fst (snd last2)) /\ Some? (ret_of last2) /\ Enqueue? (fst (snd last1)) /\
+                    eq (do (concrete_merge (v_of lca) (do (v_of s1) last1) (v_of s2')) last2)
+                       (concrete_merge (v_of lca) (do (v_of s1) last1) (do (v_of s2') last2))))
+          (ensures eq (do (concrete_merge (v_of lca) (do (v_of s1) last1) (v_of s2)) last2)
+                      (concrete_merge (v_of lca) (do (v_of s1) last1) (do (v_of s2) last2))) = 
+  admit()
+                      
+let linearizable_gt0_ind_dd_stf (lca s1 s2:st) (last1 last2:op_t)
+  : Lemma (requires consistent_branches_s2_gt0 lca s1 s2 /\
+                    fst last1 <> fst last2 /\
+                    distinct_ops (snoc (ops_of s1) last1) /\
+                    distinct_ops (snoc (ops_of s2) last2) /\
+                    (exists l1. (do (v_of s1) last1 == apply_log (v_of lca) l1)) /\
+                    (exists l2. (do (v_of s2) last2 == apply_log (v_of lca) l2)) /\
+                    (let s2' = inverse_st s2 in
+                    (exists l2. (do (v_of s2') last2 == apply_log (v_of lca) l2)) /\
+                    (exists l2. (v_of s2' == apply_log (v_of lca) l2)) /\
+                    (exists l1. (v_of s1 == apply_log (v_of lca) l1)) /\
+                    (exists l2. (v_of s2 == apply_log (v_of lca) l2)) /\
+                    consistent_branches lca s1 s2' /\
+                    ops_of s1 = ops_of lca /\
+                    Second_then_first? (resolve_conflict last1 last2) /\
+                    Dequeue? (fst (snd last1)) /\ Some? (ret_of last1) /\ 
+                    Dequeue? (fst (snd last2)) /\ Some? (ret_of last2) /\
+                    fst (extract last1) >= fst (extract last2) /\
+                    eq (do (concrete_merge (v_of lca) (do (v_of s1) last1) (v_of s2')) last2)
+                       (concrete_merge (v_of lca) (do (v_of s1) last1) (do (v_of s2') last2))))
+          (ensures eq (do (concrete_merge (v_of lca) (do (v_of s1) last1) (v_of s2)) last2)
+                      (concrete_merge (v_of lca) (do (v_of s1) last1) (do (v_of s2) last2))) = 
+   valid_is_unique lca; valid_is_unique s1; valid_is_unique s2;
+   assume (ret_of last1 = return (v_of s1) last1); //to include in pre-cond    
+   assume (ret_of last2 = return (v_of s2) last2); //to include in pre-cond  
+   last_deq (v_of s1) last1;
+   last_deq (v_of s2) last2
+
+let linearizable_gt0_ind_stf (lca s1 s2:st) (last1 last2:op_t)
+  : Lemma (requires consistent_branches_s2_gt0 lca s1 s2 /\
+                    fst last1 <> fst last2 /\
+                    distinct_ops (snoc (ops_of s1) last1) /\
+                    distinct_ops (snoc (ops_of s2) last2) /\
+                    (exists l1. (do (v_of s1) last1 == apply_log (v_of lca) l1)) /\
+                    (exists l2. (do (v_of s2) last2 == apply_log (v_of lca) l2)) /\
+                    (let s2' = inverse_st s2 in
+                    (exists l2. (do (v_of s2') last2 == apply_log (v_of lca) l2)) /\
+                    (exists l2. (v_of s2' == apply_log (v_of lca) l2)) /\
+                    (exists l1. (v_of s1 == apply_log (v_of lca) l1)) /\
+                    (exists l2. (v_of s2 == apply_log (v_of lca) l2)) /\
+                    consistent_branches lca s1 s2' /\
+                    ops_of s1 = ops_of lca /\
+                    Second_then_first? (resolve_conflict last1 last2) /\
+                    eq (do (concrete_merge (v_of lca) (do (v_of s1) last1) (v_of s2')) last2)
+                       (concrete_merge (v_of lca) (do (v_of s1) last1) (do (v_of s2') last2))))
+          (ensures eq (do (concrete_merge (v_of lca) (do (v_of s1) last1) (v_of s2)) last2)
+                      (concrete_merge (v_of lca) (do (v_of s1) last1) (do (v_of s2) last2)))
+          [SMTPat (eq (do (concrete_merge (v_of lca) (do (v_of s1) last1) (v_of s2)) last2)
+                      (concrete_merge (v_of lca) (do (v_of s1) last1) (do (v_of s2) last2)))] = 
+  if Enqueue? (fst (snd last1)) && Enqueue? (fst (snd last2)) && fst last1 < fst last2 then
+    linearizable_gt0_ind_ee_stf lca s1 s2 last1 last2
+  else if Dequeue? (fst (snd last2)) && Some? (ret_of last2) && Enqueue? (fst (snd last1)) then
+    linearizable_gt0_ind_de_stf lca s1 s2 last1 last2
+  else linearizable_gt0_ind_dd_stf lca s1 s2 last1 last2
 
 let linearizable_gt0_ind (lca s1 s2:st) (last1 last2:op_t)
   : Lemma (requires consistent_branches_s2_gt0 lca s1 s2 /\
@@ -384,7 +612,206 @@ let linearizable_gt0_ind (lca s1 s2:st) (last1 last2:op_t)
                     eq (do (concrete_merge (v_of lca) (do (v_of s1) last1) (v_of s2')) last2)
                        (concrete_merge (v_of lca) (do (v_of s1) last1) (do (v_of s2') last2))) ==>
                     (eq (do (concrete_merge (v_of lca) (do (v_of s1) last1) (v_of s2)) last2)
-                        (concrete_merge (v_of lca) (do (v_of s1) last1) (do (v_of s2) last2)))))) = admit()
+                        (concrete_merge (v_of lca) (do (v_of s1) last1) (do (v_of s2) last2)))))) = () //going thro because of SMTPat
+
+let linearizable_gt0_ind1_ee_fts (lca s1 s2:st) (last1 last2:op_t)
+  : Lemma (requires consistent_branches_s1_gt0 lca s1 s2 /\
+                    fst last1 <> fst last2 /\
+                    distinct_ops (snoc (ops_of s1) last1) /\
+                    distinct_ops (snoc (ops_of s2) last2) /\
+                    (exists l1. (do (v_of s1) last1 == apply_log (v_of lca) l1)) /\
+                    (exists l2. (do (v_of s2) last2 == apply_log (v_of lca) l2)) /\
+                    (let s1' = inverse_st s1 in
+                    (exists l1. (do (v_of s1') last1 == apply_log (v_of lca) l1)) /\
+                    (exists l1. (v_of s1' == apply_log (v_of lca) l1)) /\
+                    (exists l1. (v_of s1 == apply_log (v_of lca) l1)) /\
+                    (exists l2. (v_of s2 == apply_log (v_of lca) l2)) /\
+                    consistent_branches lca s1' s2 /\
+                    ops_of s2 = ops_of lca /\
+                    First_then_second? (resolve_conflict last1 last2) /\
+                    Enqueue? (fst (snd last1)) /\ Enqueue? (fst (snd last2)) /\ fst last1 > fst last2 /\
+                    eq (do (concrete_merge (v_of lca) (v_of s1') (do (v_of s2) last2)) last1)
+                       (concrete_merge (v_of lca) (do (v_of s1') last1) (do (v_of s2) last2))))
+          (ensures eq (do (concrete_merge (v_of lca) (v_of s1) (do (v_of s2) last2)) last1)
+                      (concrete_merge (v_of lca) (do (v_of s1) last1) (do (v_of s2) last2))) = ()
+
+let linearizable_gt0_ind1_de_fts (lca s1 s2:st) (last1 last2:op_t)
+  : Lemma (requires consistent_branches_s1_gt0 lca s1 s2 /\
+                    fst last1 <> fst last2 /\
+                    distinct_ops (snoc (ops_of s1) last1) /\
+                    distinct_ops (snoc (ops_of s2) last2) /\
+                    (exists l1. (do (v_of s1) last1 == apply_log (v_of lca) l1)) /\
+                    (exists l2. (do (v_of s2) last2 == apply_log (v_of lca) l2)) /\
+                    (let s1' = inverse_st s1 in
+                    (exists l1. (do (v_of s1') last1 == apply_log (v_of lca) l1)) /\
+                    (exists l1. (v_of s1' == apply_log (v_of lca) l1)) /\
+                    (exists l1. (v_of s1 == apply_log (v_of lca) l1)) /\
+                    (exists l2. (v_of s2 == apply_log (v_of lca) l2)) /\
+                    consistent_branches lca s1' s2 /\
+                    ops_of s2 = ops_of lca /\
+                    First_then_second? (resolve_conflict last1 last2) /\
+                    Dequeue? (fst (snd last1)) /\ Some? (ret_of last1) /\ Enqueue? (fst (snd last2)) /\
+                    eq (do (concrete_merge (v_of lca) (v_of s1') (do (v_of s2) last2)) last1)
+                       (concrete_merge (v_of lca) (do (v_of s1') last1) (do (v_of s2) last2))))
+          (ensures eq (do (concrete_merge (v_of lca) (v_of s1) (do (v_of s2) last2)) last1)
+                      (concrete_merge (v_of lca) (do (v_of s1) last1) (do (v_of s2) last2))) = admit()
+
+let linearizable_gt0_ind1_dd_fts (lca s1 s2:st) (last1 last2:op_t)
+  : Lemma (requires consistent_branches_s1_gt0 lca s1 s2 /\
+                    fst last1 <> fst last2 /\
+                    distinct_ops (snoc (ops_of s1) last1) /\
+                    distinct_ops (snoc (ops_of s2) last2) /\
+                    (exists l1. (do (v_of s1) last1 == apply_log (v_of lca) l1)) /\
+                    (exists l2. (do (v_of s2) last2 == apply_log (v_of lca) l2)) /\
+                    (let s1' = inverse_st s1 in
+                    (exists l1. (do (v_of s1') last1 == apply_log (v_of lca) l1)) /\
+                    (exists l1. (v_of s1' == apply_log (v_of lca) l1)) /\
+                    (exists l1. (v_of s1 == apply_log (v_of lca) l1)) /\
+                    (exists l2. (v_of s2 == apply_log (v_of lca) l2)) /\
+                    consistent_branches lca s1' s2 /\
+                    ops_of s2 = ops_of lca /\
+                    First_then_second? (resolve_conflict last1 last2) /\
+                    Dequeue? (fst (snd last1)) /\ Some? (ret_of last1) /\ 
+                    Dequeue? (fst (snd last2)) /\ Some? (ret_of last2) /\
+                    fst (extract last1) < fst (extract last2) /\
+                    eq (do (concrete_merge (v_of lca) (v_of s1') (do (v_of s2) last2)) last1)
+                       (concrete_merge (v_of lca) (do (v_of s1') last1) (do (v_of s2) last2))))
+          (ensures eq (do (concrete_merge (v_of lca) (v_of s1) (do (v_of s2) last2)) last1)
+                      (concrete_merge (v_of lca) (do (v_of s1) last1) (do (v_of s2) last2))) = 
+   valid_is_unique lca; valid_is_unique s1; valid_is_unique s2;
+   assume (ret_of last1 = return (v_of s1) last1); //to include in pre-cond    
+   assume (ret_of last2 = return (v_of s2) last2); //to include in pre-cond  
+   last_deq (v_of s1) last1;
+   last_deq (v_of s2) last2
+
+let linearizable_gt0_ind1_fts (lca s1 s2:st) (last1 last2:op_t)
+  : Lemma (requires consistent_branches_s1_gt0 lca s1 s2 /\
+                    fst last1 <> fst last2 /\
+                    distinct_ops (snoc (ops_of s1) last1) /\
+                    distinct_ops (snoc (ops_of s2) last2) /\
+                    (exists l1. (do (v_of s1) last1 == apply_log (v_of lca) l1)) /\
+                    (exists l2. (do (v_of s2) last2 == apply_log (v_of lca) l2)) /\
+                    (let s1' = inverse_st s1 in
+                    (exists l1. (do (v_of s1') last1 == apply_log (v_of lca) l1)) /\
+                    (exists l1. (v_of s1' == apply_log (v_of lca) l1)) /\
+                    (exists l1. (v_of s1 == apply_log (v_of lca) l1)) /\
+                    (exists l2. (v_of s2 == apply_log (v_of lca) l2)) /\
+                    consistent_branches lca s1' s2 /\
+                    ops_of s2 = ops_of lca /\
+                    First_then_second? (resolve_conflict last1 last2) /\
+                    eq (do (concrete_merge (v_of lca) (v_of s1') (do (v_of s2) last2)) last1)
+                       (concrete_merge (v_of lca) (do (v_of s1') last1) (do (v_of s2) last2))))
+          (ensures eq (do (concrete_merge (v_of lca) (v_of s1) (do (v_of s2) last2)) last1)
+                      (concrete_merge (v_of lca) (do (v_of s1) last1) (do (v_of s2) last2)))
+          [SMTPat (eq (do (concrete_merge (v_of lca) (v_of s1) (do (v_of s2) last2)) last1)
+                      (concrete_merge (v_of lca) (do (v_of s1) last1) (do (v_of s2) last2)))] = 
+  if Enqueue? (fst (snd last1)) && Enqueue? (fst (snd last2)) && fst last1 > fst last2 then
+    linearizable_gt0_ind1_ee_fts lca s1 s2 last1 last2
+  else if Dequeue? (fst (snd last1)) && Some? (ret_of last1) && Enqueue? (fst (snd last2)) then
+    linearizable_gt0_ind1_de_fts lca s1 s2 last1 last2
+  else linearizable_gt0_ind1_dd_fts lca s1 s2 last1 last2
+
+let linearizable_gt0_ind1_ee_stf (lca s1 s2:st) (last1 last2:op_t)
+  : Lemma (requires consistent_branches_s1_gt0 lca s1 s2 /\
+                    fst last1 <> fst last2 /\
+                    distinct_ops (snoc (ops_of s1) last1) /\
+                    distinct_ops (snoc (ops_of s2) last2) /\
+                    (exists l1. (do (v_of s1) last1 == apply_log (v_of lca) l1)) /\
+                    (exists l2. (do (v_of s2) last2 == apply_log (v_of lca) l2)) /\
+                    (let s1' = inverse_st s1 in
+                    (exists l1. (do (v_of s1') last1 == apply_log (v_of lca) l1)) /\
+                    (exists l1. (v_of s1' == apply_log (v_of lca) l1)) /\
+                    (exists l1. (v_of s1 == apply_log (v_of lca) l1)) /\
+                    (exists l2. (v_of s2 == apply_log (v_of lca) l2)) /\
+                    consistent_branches lca s1' s2 /\
+                    Second_then_first? (resolve_conflict last1 last2) /\
+                    Enqueue? (fst (snd last1)) /\ Enqueue? (fst (snd last2)) /\ fst last1 < fst last2 /\
+                    eq (do (concrete_merge (v_of lca) (do (v_of s1') last1) (v_of s2)) last2)
+                       (concrete_merge (v_of lca) (do (v_of s1') last1) (do (v_of s2) last2))))
+          (ensures eq (do (concrete_merge (v_of lca) (do (v_of s1) last1) (v_of s2)) last2)
+                      (concrete_merge (v_of lca) (do (v_of s1) last1) (do (v_of s2) last2))) = 
+  assume (forall id. S.mem_id_s id (v_of lca) ==> fst last2 > id); //todo
+  ()
+
+let linearizable_gt0_ind1_de_stf (lca s1 s2:st) (last1 last2:op_t)
+  : Lemma (requires consistent_branches_s1_gt0 lca s1 s2 /\
+                    fst last1 <> fst last2 /\
+                    distinct_ops (snoc (ops_of s1) last1) /\
+                    distinct_ops (snoc (ops_of s2) last2) /\
+                    (exists l1. (do (v_of s1) last1 == apply_log (v_of lca) l1)) /\
+                    (exists l2. (do (v_of s2) last2 == apply_log (v_of lca) l2)) /\
+                    (let s1' = inverse_st s1 in
+                    (exists l1. (do (v_of s1') last1 == apply_log (v_of lca) l1)) /\
+                    (exists l1. (v_of s1' == apply_log (v_of lca) l1)) /\
+                    (exists l1. (v_of s1 == apply_log (v_of lca) l1)) /\
+                    (exists l2. (v_of s2 == apply_log (v_of lca) l2)) /\
+                    consistent_branches lca s1' s2 /\
+                    Second_then_first? (resolve_conflict last1 last2) /\
+                    Dequeue? (fst (snd last2)) /\ Some? (ret_of last2) /\ Enqueue? (fst (snd last1)) /\
+                    eq (do (concrete_merge (v_of lca) (do (v_of s1') last1) (v_of s2)) last2)
+                       (concrete_merge (v_of lca) (do (v_of s1') last1) (do (v_of s2) last2))))
+          (ensures eq (do (concrete_merge (v_of lca) (do (v_of s1) last1) (v_of s2)) last2)
+                      (concrete_merge (v_of lca) (do (v_of s1) last1) (do (v_of s2) last2))) = admit()
+
+let linearizable_gt0_ind1_dd_stf (lca s1 s2:st) (last1 last2:op_t)
+  : Lemma (requires consistent_branches_s1_gt0 lca s1 s2 /\
+                    fst last1 <> fst last2 /\
+                    distinct_ops (snoc (ops_of s1) last1) /\
+                    distinct_ops (snoc (ops_of s2) last2) /\
+                    (exists l1. (do (v_of s1) last1 == apply_log (v_of lca) l1)) /\
+                    (exists l2. (do (v_of s2) last2 == apply_log (v_of lca) l2)) /\
+                    (let s1' = inverse_st s1 in
+                    (exists l1. (do (v_of s1') last1 == apply_log (v_of lca) l1)) /\
+                    (exists l1. (v_of s1' == apply_log (v_of lca) l1)) /\
+                    (exists l1. (v_of s1 == apply_log (v_of lca) l1)) /\
+                    (exists l2. (v_of s2 == apply_log (v_of lca) l2)) /\
+                    consistent_branches lca s1' s2 /\
+                    Second_then_first? (resolve_conflict last1 last2) /\
+                    Dequeue? (fst (snd last1)) /\ Some? (ret_of last1) /\ 
+                    Dequeue? (fst (snd last2)) /\ Some? (ret_of last2) /\
+                    fst (extract last1) >= fst (extract last2) /\
+                    eq (do (concrete_merge (v_of lca) (do (v_of s1') last1) (v_of s2)) last2)
+                       (concrete_merge (v_of lca) (do (v_of s1') last1) (do (v_of s2) last2))))
+          (ensures eq (do (concrete_merge (v_of lca) (do (v_of s1) last1) (v_of s2)) last2)
+                      (concrete_merge (v_of lca) (do (v_of s1) last1) (do (v_of s2) last2))) = 
+  valid_is_unique lca; valid_is_unique s1; valid_is_unique s2;
+  assume (ret_of last1 = return (v_of s1) last1); //to include in pre-cond    
+  assume (ret_of last2 = return (v_of s2) last2); //to include in pre-cond  
+  last_deq (v_of s1) last1;
+  last_deq (v_of s2) last2;
+     //assume (forall e. S.mem e (v_of s1) /\ S.mem e (do (v_of s2) last2) ==> S.mem e (v_of lca));
+     //assume (forall e. S.mem e (do (v_of s1) last1) /\ S.mem e (do (v_of s2) last2) ==> S.mem e (v_of lca));
+     //assume (fst (extract_s (find_min (v_of s1))) < fst (extract_s (find_min (v_of s2))));
+  let s1' = inverse_st s1 in
+  assume (S.find_min (concrete_merge (v_of lca) (do (v_of s1') last1) (do (v_of s2) last2)) = (S.find_min (v_of s2)));
+  assert (S.find_min (concrete_merge (v_of lca) (do (v_of s1) last1) (v_of s2)) = (S.find_min (v_of s2)));
+  ()
+
+let linearizable_gt0_ind1_stf (lca s1 s2:st) (last1 last2:op_t)
+  : Lemma (requires consistent_branches_s1_gt0 lca s1 s2 /\
+                    fst last1 <> fst last2 /\
+                    distinct_ops (snoc (ops_of s1) last1) /\
+                    distinct_ops (snoc (ops_of s2) last2) /\
+                    (exists l1. (do (v_of s1) last1 == apply_log (v_of lca) l1)) /\
+                    (exists l2. (do (v_of s2) last2 == apply_log (v_of lca) l2)) /\
+                    (let s1' = inverse_st s1 in
+                    (exists l1. (do (v_of s1') last1 == apply_log (v_of lca) l1)) /\
+                    (exists l1. (v_of s1' == apply_log (v_of lca) l1)) /\
+                    (exists l1. (v_of s1 == apply_log (v_of lca) l1)) /\
+                    (exists l2. (v_of s2 == apply_log (v_of lca) l2)) /\
+                    consistent_branches lca s1' s2 /\
+                    Second_then_first? (resolve_conflict last1 last2) /\
+                    eq (do (concrete_merge (v_of lca) (do (v_of s1') last1) (v_of s2)) last2)
+                       (concrete_merge (v_of lca) (do (v_of s1') last1) (do (v_of s2) last2))))
+          (ensures eq (do (concrete_merge (v_of lca) (do (v_of s1) last1) (v_of s2)) last2)
+                      (concrete_merge (v_of lca) (do (v_of s1) last1) (do (v_of s2) last2))) 
+          [SMTPat (eq (do (concrete_merge (v_of lca) (do (v_of s1) last1) (v_of s2)) last2)
+                      (concrete_merge (v_of lca) (do (v_of s1) last1) (do (v_of s2) last2)))] =  
+  if Enqueue? (fst (snd last1)) && Enqueue? (fst (snd last2)) && fst last1 < fst last2 then
+    linearizable_gt0_ind1_ee_stf lca s1 s2 last1 last2
+  else if Dequeue? (fst (snd last2)) && Some? (ret_of last2) && Enqueue? (fst (snd last1)) then
+    linearizable_gt0_ind1_de_stf lca s1 s2 last1 last2
+  else linearizable_gt0_ind1_dd_stf lca s1 s2 last1 last2
 
 let linearizable_gt0_ind1 (lca s1 s2:st) (last1 last2:op_t)
   : Lemma (requires consistent_branches_s1_gt0 lca s1 s2 /\
@@ -412,7 +839,33 @@ let linearizable_gt0_ind1 (lca s1 s2:st) (last1 last2:op_t)
                     eq (do (concrete_merge (v_of lca) (do (v_of s1') last1) (v_of s2)) last2)
                        (concrete_merge (v_of lca) (do (v_of s1') last1) (do (v_of s2) last2)) ==>
                     eq (do (concrete_merge (v_of lca) (do (v_of s1) last1) (v_of s2)) last2)
-                       (concrete_merge (v_of lca) (do (v_of s1) last1) (do (v_of s2) last2)))))) = admit()
+                       (concrete_merge (v_of lca) (do (v_of s1) last1) (do (v_of s2) last2)))))) = ()
+
+let rec lem_s1s2_then_lca (lca s1 s2:st)
+  : Lemma (requires consistent_branches lca s1 s2)
+          (ensures (forall e. S.mem e (v_of s1) /\ S.mem e (v_of s2) ==> S.mem e (v_of lca)))
+          (decreases %[(length (ops_of s1))]) =
+  if ops_of s1 = ops_of lca && ops_of s2 = ops_of lca then ()
+  else if ops_of s1 = ops_of lca then ()
+  else (let s1' = inverse_st s1 in
+        let pre1, last1 = un_snoc (ops_of s1) in
+        lemma_mem_snoc pre1 last1;
+        distinct_invert_append pre1 (create 1 last1);
+        lem_inverse (ops_of lca) (ops_of s1); 
+        lastop_diff (ops_of lca) (ops_of s1);
+        inverse_diff_id_s1' (ops_of lca) (ops_of s1) (ops_of s2);
+        if Dequeue? (fst (snd last1)) then
+          (lem_s1s2_then_lca lca s1' s2;
+           valid_is_unique lca; valid_is_unique s1; valid_is_unique s2; valid_is_unique s1')
+        else (lem_s1s2_then_lca lca s1' s2;
+              valid_is_unique lca; valid_is_unique s1; valid_is_unique s2; valid_is_unique s1';
+              lem_foldl init_st (ops_of lca); lem_foldl init_st (ops_of s1); lem_foldl init_st (ops_of s2); 
+              split_prefix init_st (ops_of lca) (ops_of s1); 
+              lem_foldl (v_of lca) (diff (ops_of s1) (ops_of lca));
+              split_prefix init_st (ops_of lca) (ops_of s2);
+              lem_foldl (v_of lca) (diff (ops_of s2) (ops_of lca));
+              lem_diff (ops_of s1) (ops_of lca); 
+              lastop_diff (ops_of lca) (ops_of s1)))
 
 let linearizable_gt0_s1's2' (lca s1 s2:st)
   : Lemma (requires consistent_branches_s1s2_gt0 lca s1 s2 /\ 
@@ -429,10 +882,28 @@ let linearizable_gt0_s1's2' (lca s1 s2:st)
           (ensures (let _, last1 = un_snoc (ops_of s1) in
                     eq (do (concrete_merge (v_of lca) (v_of (inverse_st s1)) (v_of (inverse_st s2))) last1)
                        (concrete_merge (v_of lca) (v_of s1) (v_of s2)))) = 
-   assume (unique_st (v_of lca) /\ unique_st (v_of s1) /\ unique_st (v_of s2)); //todo
+   let _, last1 = un_snoc (ops_of s1) in
+   let _, last2 = un_snoc (ops_of s2) in
+   valid_is_unique lca; valid_is_unique s1; valid_is_unique s2; 
+   valid_is_unique (inverse_st s1); valid_is_unique (inverse_st s2);
    lem_apply_log init_st (ops_of s1);
    lem_apply_log init_st (ops_of s2);
-   admit()
+   last_deq (v_of (inverse_st s1)) last1;
+   last_deq (v_of (inverse_st s2)) last2;
+   assume (consistent_branches lca (inverse_st s1) (inverse_st s2)); //can be done
+   lem_s1s2_then_lca lca (inverse_st s1) (inverse_st s2);
+   assert (forall e. S.mem e (v_of (inverse_st s1)) /\ S.mem e (v_of (inverse_st s2)) ==> S.mem e (v_of lca));
+   let i' = S.intersect (v_of lca) (S.intersect (v_of (inverse_st s1)) (v_of (inverse_st s2))) in
+   let i = S.intersect (v_of lca)  (S.intersect (v_of s1) (v_of s2)) in
+   assert (forall e. S.mem e i <==> S.mem e i' /\ e <> S.extract_s (S.find_min (v_of (inverse_st s1)))); 
+   let da' = S.remove_if (v_of (inverse_st s1)) (fun e -> S.mem e (v_of lca)) in
+   let db' = S.remove_if (v_of (inverse_st s2)) (fun e -> S.mem e (v_of lca)) in
+   let da = S.remove_if (v_of s1) (fun e -> S.mem e (v_of lca)) in
+   let db = S.remove_if (v_of s2) (fun e -> S.mem e (v_of lca)) in
+   assert (eq da' da);
+   assert (eq db' db); 
+   ()
+#pop-options
 
 let linearizable_gt0_s1'_noop (lca s1 s2:st)
   : Lemma (requires consistent_branches_s1s2_gt0 lca s1 s2 /\ 
@@ -446,7 +917,7 @@ let linearizable_gt0_s1'_noop (lca s1 s2:st)
                      is_prefix (ops_of lca) (ops_of (inverse_st s1))))
           (ensures eq (concrete_merge (v_of lca) (v_of (inverse_st s1)) (v_of s2))
                       (concrete_merge (v_of lca) (v_of s1) (v_of s2))) = 
-  assume (unique_st (v_of lca) /\ unique_st (v_of s1) /\ unique_st (v_of s2)); //todo
+  valid_is_unique lca; valid_is_unique s1; valid_is_unique s2;
   lem_apply_log init_st (ops_of s1)
 
 let linearizable_gt0_s2'_noop (lca s1 s2:st)
@@ -461,7 +932,7 @@ let linearizable_gt0_s2'_noop (lca s1 s2:st)
                      is_prefix (ops_of lca) (ops_of (inverse_st s2))))
           (ensures eq (concrete_merge (v_of lca) (v_of s1) (v_of (inverse_st s2)))
                       (concrete_merge (v_of lca) (v_of s1) (v_of s2))) = 
-  assume (unique_st (v_of lca) /\ unique_st (v_of s1) /\ unique_st (v_of s2)); //todo
+  valid_is_unique lca; valid_is_unique s1; valid_is_unique s2;
   lem_apply_log init_st (ops_of s2)
   
 let linearizable_gt0_s1's2'_noop_both (lca s1 s2:st)
@@ -492,18 +963,18 @@ let init_st_s = S.empty
 let find_min_seq (s:concrete_st_s)
     : (m:option nat
            {(Some? m <==> (exists (e:(nat)). S.mem e s /\ (forall e1. S.mem e1 s ==> e <= e1))) /\
-            (Some? m ==> (exists (e:(nat)). S.mem e s /\ (forall e1. S.mem e1 s ==> e <= e1) /\ e = extract_s m)) /\
+            (Some? m ==> (exists (e:(nat)). S.mem e s /\ (forall e1. S.mem e1 s ==> e <= e1) /\ e = S.extract_s m)) /\
         (s = S.empty ==> (m = None \/ (~ (exists (e:(nat)). S.mem e s /\ (forall e1. S.mem e1 s ==> e <= e1))))) 
         (*s <> empty ==> Some? m*)}) =
   S.find_if s (fun e -> (S.forall_s s (fun e1 -> e <= e1)))
   
 let remove_min_seq (s:concrete_st_s) 
   : (r:concrete_st_s{(s = S.empty ==> r = s) /\
-                   (s <> S.empty /\ Some? (find_min_seq s) ==> (forall e. S.mem e r <==> (S.mem e s /\ e <> extract_s (find_min_seq s)))) /\
+                   (s <> S.empty /\ Some? (find_min_seq s) ==> (forall e. S.mem e r <==> (S.mem e s /\ e <> S.extract_s (find_min_seq s)))) /\
                    (s <> S.empty /\ None? (find_min_seq s) ==> (forall e. S.mem e r <==> S.mem e s))}) =
   if s = S.empty then s 
   else (let m = find_min_seq s in
-        if Some? m then S.remove_if s (fun e -> e = extract_s (find_min_seq s))
+        if Some? m then S.remove_if s (fun e -> e = S.extract_s (find_min_seq s))
         else s)
         
 // apply an operation to a state 
@@ -523,14 +994,14 @@ let initial_eq _
 
 let min_same (st_s:concrete_st_s) (st:concrete_st) 
   : Lemma (requires eq_sm st_s st)
-          (ensures (None? (find_min_seq st_s) <==> None? (find_min st)) /\
-                   (Some? (find_min_seq st_s) <==> Some? (find_min st)) /\
-                   (Some? (find_min_seq st_s) ==> extract_s (find_min_seq st_s) = snd (extract_s (find_min st)))) = admit()
+          (ensures (None? (find_min_seq st_s) <==> None? (S.find_min st)) /\
+                   (Some? (find_min_seq st_s) <==> Some? (S.find_min st)) /\
+                   (Some? (find_min_seq st_s) ==> S.extract_s (find_min_seq st_s) = snd (S.extract_s (S.find_min st)))) = admit()
 
 let remove_same (st_s:concrete_st_s) (st:concrete_st) 
   : Lemma (requires eq_sm st_s st)
-          (ensures (eq_sm (remove_min_seq st_s) (remove_min st))) =
-  admit();min_same st_s st
+          (ensures (eq_sm (remove_min_seq st_s) (S.remove_min st))) =
+  admit()
  
 //equivalence between states of sequential type and MRDT at every operation
 let do_eq (st_s:concrete_st_s) (st:concrete_st) (op:op_t)
