inductive_proof/Queue_set/Set_extended.fsti
@@ -80,3 +80,35 @@ val mem_find_if_exists (#a:eqtype) (s:set a) (f:a -> bool)
                    (Some? (find_if s f) ==> (exists e. mem e s /\ f e /\ e = extr (find_if s f)) /\ (f (extr (find_if s f)))) /\
                    (s <> empty ==> Some? (find_if s f)))
           [SMTPat (find_if s f)]
+
+val always_min_exists (#a:eqtype) (s:set (nat * a)) 
+  : Lemma (ensures (s <> empty ==> (exists (e:(nat * a)). mem e s /\ (forall (e1:(nat * a)). mem e1 s ==> fst e <= fst e1))))
+
+val extract_s (#a:Type0) (m:option a{Some? m}) : (e:a{m == Some e})
+
+val find_min (#a:eqtype) (s:set (nat * a)) 
+  : (m:option (nat * a)
+     {(Some? m <==> (exists (e:(nat * a)). mem e s /\ (forall e1. mem e1 s ==> fst e <= fst e1))) /\
+            (Some? m ==> (exists (e:(nat * a)). mem e s /\ (forall e1. mem e1 s ==> fst e <= fst e1) /\ e = extract_s m)) /\
+        (s = empty ==> (m = None \/ (~ (exists (e:(nat * a)). mem e s /\ (forall e1. mem e1 s ==> fst e <= fst e1))))) })
+
+val mem_find_min (#a:eqtype) (s:set (nat * a))
+  : Lemma (ensures (Some? (find_min s) <==> (exists (e:(nat * a)). mem e s /\ (forall e1. mem e1 s ==> fst e <= fst e1))) /\
+            (Some? (find_min s) ==> (exists (e:(nat * a)). mem e s /\ (forall e1. mem e1 s ==> fst e <= fst e1) /\ e = extract_s (find_min s))) /\
+        (s = empty ==> (find_min s = None \/ (~ (exists (e:(nat * a)). mem e s /\ (forall e1. mem e1 s ==> fst e <= fst e1)))))) 
+        [SMTPat (find_min s)]
+
+let unique_st (#a:eqtype) (s:set (nat * a)) =
+  forall_s s (fun e -> not (exists_s s (fun e1 -> snd e <> snd e1 && fst e = fst e1)))
+
+val remove_min (#a:eqtype) (s:set (nat * a)) 
+  : (r:set (nat * a){(s = empty ==> r = s) /\
+                   (s <> empty /\ Some? (find_min s) ==> (forall e. mem e r <==> (mem e s /\ e <> extract_s (find_min s)))) /\
+                   (s <> empty /\ None? (find_min s) ==> (forall e. mem e r <==> mem e s))})
+
+val mem_id_s (#a:eqtype) (id:nat) (s:set (nat * a)) 
+  : (b:bool{b = true <==> (exists e. mem e s /\ fst e = id)})
+
+val eq_min_same (#a:eqtype) (s1 s2:set (nat * a))
+  : Lemma (requires equal s1 s2 /\ unique_st s1 /\ unique_st s2)
+          (ensures find_min s1 = find_min s2)
